backend/RTLC.v
@@ -23,78 +23,60 @@ Section MODSEM.
   | at_external_intro
       stack fptr_arg sg_arg vs_arg m0
       (EXTERNAL: ge.(Genv.find_funct) fptr_arg = None)
-      (SIG: exists skd, skenv_link.(Genv.find_funct) fptr_arg = Some skd /\ SkEnv.get_sig skd = sg_arg)
-    :
-      at_external (Callstate stack fptr_arg sg_arg vs_arg m0) (Args.mk fptr_arg vs_arg m0)
-  .
+      (SIG: exists skd, skenv_link.(Genv.find_funct) fptr_arg = Some skd /\ SkEnv.get_sig skd = sg_arg):
+      at_external (Callstate stack fptr_arg sg_arg vs_arg m0) (Args.mk fptr_arg vs_arg m0).
 
-  Inductive initial_frame (args: Args.t)
-    : state -> Prop :=
+  Inductive initial_frame (args: Args.t): state -> Prop :=
   | initial_frame_intro
       fd tvs
       (FINDF: Genv.find_funct ge args.(Args.fptr) = Some (Internal fd))
       (TYP: typecheck args.(Args.vs) fd.(fn_sig) tvs)
-      (LEN: args.(Args.vs).(length) = fd.(fn_sig).(sig_args).(length))
-    :
-      initial_frame args (Callstate [] args.(Args.fptr) fd.(fn_sig) tvs args.(Args.m))
-  .
+      (LEN: args.(Args.vs).(length) = fd.(fn_sig).(sig_args).(length)):
+      initial_frame args (Callstate [] args.(Args.fptr) fd.(fn_sig) tvs args.(Args.m)).
 
-  Inductive initial_frame2 (args: Args.t)
-    : state -> Prop :=
+  Inductive initial_frame2 (args: Args.t): state -> Prop :=
   | initial_frame2_intro
-      fd tvs
+      fd tvs n m0
       (FINDF: Genv.find_funct ge args.(Args.fptr) = Some (Internal fd))
       (TYP: typecheck args.(Args.vs) fd.(fn_sig) tvs)
       (LEN: args.(Args.vs).(length) = fd.(fn_sig).(sig_args).(length))
-      n m0
-      (JUNK: assign_junk_blocks args.(Args.m) n = m0)
-    :
-      initial_frame2 args (Callstate [] args.(Args.fptr) fd.(fn_sig) tvs m0)
-  .
+      (JUNK: assign_junk_blocks args.(Args.m) n = m0):
+      initial_frame2 args (Callstate [] args.(Args.fptr) fd.(fn_sig) tvs m0).
 
   Inductive final_frame: state -> Retv.t -> Prop :=
   | final_frame_intro
-      v_ret m_ret
-    :
-      final_frame (Returnstate [] v_ret m_ret) (Retv.mk v_ret m_ret)
-  .
+      v_ret m_ret:
+      final_frame (Returnstate [] v_ret m_ret) (Retv.mk v_ret m_ret).
 
   Inductive after_external: state -> Retv.t -> state -> Prop :=
   | after_external_intro
-      stack fptr_arg sg_arg vs_arg m_arg
-      retv tv
-      (TYP: typify retv.(Retv.v) sg_arg.(proj_sig_res) = tv)
-    :
+      stack fptr_arg sg_arg vs_arg m_arg retv tv
+      (TYP: typify retv.(Retv.v) sg_arg.(proj_sig_res) = tv):
       after_external (Callstate stack fptr_arg sg_arg vs_arg m_arg)
                      retv
-                     (Returnstate stack tv retv.(Retv.m))
-  .
+                     (Returnstate stack tv retv.(Retv.m)).
 
   Program Definition modsem: ModSem.t :=
-    {|
-      ModSem.step := step;
-      ModSem.at_external := at_external;
-      ModSem.initial_frame := initial_frame;
-      ModSem.final_frame := final_frame;
-      ModSem.after_external := after_external;
-      ModSem.globalenv := ge;
-      ModSem.skenv := skenv; 
-      ModSem.skenv_link := skenv_link; 
-    |}
-  .
+    {| ModSem.step := step;
+       ModSem.at_external := at_external;
+       ModSem.initial_frame := initial_frame;
+       ModSem.final_frame := final_frame;
+       ModSem.after_external := after_external;
+       ModSem.globalenv := ge;
+       ModSem.skenv := skenv; 
+       ModSem.skenv_link := skenv_link; 
+    |}.
 
   Program Definition modsem2: ModSem.t :=
-    {|
-      ModSem.step := step;
-      ModSem.at_external := at_external;
-      ModSem.initial_frame := initial_frame2;
-      ModSem.final_frame := final_frame;
-      ModSem.after_external := after_external;
-      ModSem.globalenv := ge;
-      ModSem.skenv := skenv; 
-      ModSem.skenv_link := skenv_link; 
-    |}
-  .
+    {| ModSem.step := step;
+       ModSem.at_external := at_external;
+       ModSem.initial_frame := initial_frame2;
+       ModSem.final_frame := final_frame;
+       ModSem.after_external := after_external;
+       ModSem.globalenv := ge;
+       ModSem.skenv := skenv; 
+       ModSem.skenv_link := skenv_link; 
+    |}.
 
   Lemma modsem_receptive: forall st, receptive_at modsem st.
     econs; eauto.
@@ -110,13 +92,17 @@ Section MODSEM.
 
   Lemma modsem_determinate: forall st, determinate_at modsem st.
     econs; eauto.
-    - ii; ss. inv H; inv H0; clarify_meq; try (determ_tac eval_builtin_args_determ; check_safe); try (determ_tac external_call_determ; check_safe); esplits; eauto; try (econs; eauto); ii; eq_closure_tac; clarify_meq.
+    - ii; ss. inv H; inv H0; clarify_meq; try (determ_tac eval_builtin_args_determ; check_safe);
+                try (determ_tac external_call_determ; check_safe);
+                esplits; eauto; try (econs; eauto); ii; eq_closure_tac; clarify_meq.
     - ii. inv H; try (exploit external_call_trace_length; eauto; check_safe; intro T; des); ss; try xomega.
   Qed.
 
   Lemma modsem2_determinate: forall st, determinate_at modsem2 st.
     econs; eauto.
-    - ii; ss. inv H; inv H0; clarify_meq; try (determ_tac eval_builtin_args_determ; check_safe); try (determ_tac external_call_determ; check_safe); esplits; eauto; try (econs; eauto); ii; eq_closure_tac; clarify_meq.
+    - ii; ss. inv H; inv H0; clarify_meq; try (determ_tac eval_builtin_args_determ; check_safe);
+                try (determ_tac external_call_determ; check_safe);
+                esplits; eauto;try (econs; eauto); ii; eq_closure_tac; clarify_meq.
     - ii. inv H; try (exploit external_call_trace_length; eauto; check_safe; intro T; des); ss; try xomega.
   Qed.
 
