backend/UnusedglobproofC.v
@@ -23,8 +23,7 @@ Section SIMMODSEM.
 
 Variable skenv_link_src skenv_link_tgt: SkEnv.t.
 Variable sm_link: SimMem.t.
-Variable prog: RTL.program.
-Variable tprog: RTL.program.
+Variable prog tprog: RTL.program.
 Let md_src: Mod.t := (RTLC.module prog).
 Let md_tgt: Mod.t := (RTLC.module2 tprog).
 Hypothesis (INCLSRC: SkEnv.includes skenv_link_src md_src.(Mod.sk)).
@@ -37,8 +36,7 @@ Let tge := (SkEnv.revive (SkEnv.project skenv_link_tgt md_tgt.(Mod.sk)) tprog).
 Definition msp: ModSemPair.t :=
   ModSemPair.mk (md_src.(Mod.modsem) skenv_link_src) (md_tgt.(Mod.modsem) skenv_link_tgt)
                 ((prog.(defs) -1 tprog.(defs) -1 (Pos.eq_dec tprog.(prog_main))): ident -> Prop)
-                sm_link
-.
+                sm_link.
 
 Inductive match_states
           (sm_init: SimMem.t)
@@ -46,21 +44,16 @@ Inductive match_states
 | match_states_intro
     (MATCHST: Unusedglobproof.match_states prog tprog (used_set tprog) skenv_link_src skenv_link_tgt ge tge st_src0 st_tgt0 sm0)
     (MCOMPATSRC: st_src0.(RTL.get_mem) = sm0.(SimMem.src))
-    (MCOMPATTGT: st_tgt0.(RTL.get_mem) = sm0.(SimMem.tgt))
-.
+    (MCOMPATTGT: st_tgt0.(RTL.get_mem) = sm0.(SimMem.tgt)).
 
 Lemma find_funct_inject
       used fptr tfptr fd j
       (SIMGE: meminj_preserves_globals prog tprog used ge tge j)
       (FINDSRC: Genv.find_funct ge fptr = Some fd)
-      (INJ: Val.inject j fptr tfptr)
-  :
-    <<FINDTGT: Genv.find_funct tge tfptr = Some fd>>
-.
+      (INJ: Val.inject j fptr tfptr):
+    <<FINDTGT: Genv.find_funct tge tfptr = Some fd>>.
 Proof.
-  inv SIMGE.
-  uge0. des_ifs_safe.
-  inv INJ.
+  inv SIMGE. uge0. des_ifs_safe. inv INJ.
   exploit defs_inject; et. i; des. clarify. psimpl. des_ifs.
 Qed.
 
@@ -69,14 +62,11 @@ Theorem sim_skenv_meminj_preserves_globals
         (SIMSKENV:
            SimSymbDrop.sim_skenv
              sm_arg ((prog.(defs) -1 tprog.(defs) -1 (Pos.eq_dec tprog.(prog_main))): ident -> Prop)
-             (SkEnv.project skenv_link_src md_src.(Mod.sk)) (SkEnv.project skenv_link_tgt md_tgt.(Mod.sk)))
-  :
-    <<SIMGE: meminj_preserves_globals prog tprog (used_set tprog) ge tge (SimMemInj.inj sm_arg)>>
-.
+             (SkEnv.project skenv_link_src md_src.(Mod.sk)) (SkEnv.project skenv_link_tgt md_tgt.(Mod.sk))):
+    <<SIMGE: meminj_preserves_globals prog tprog (used_set tprog) ge tge (SimMemInj.inj sm_arg)>>.
 Proof.
   inv SIMSKENV. ss. bar.
-  destruct TRANSL as [used0 TRANSL0]. desH TRANSL0. clarify.
-  econs.
+  destruct TRANSL as [used0 TRANSL0]. desH TRANSL0. clarify. econs.
   - i. exploit SIMSYMB1; et. i; des. clarify.
   - i. exploit SIMSYMB2; et.
     { ii. des. unfold used_set in *. ss. des_sumbool.
@@ -110,8 +100,7 @@ Proof.
       erewrite match_prog_def; et. des_ifs.
       (* exploit IS.mem_1; et. i; clarify. *)
     + i. eapply used_closed; et.
-  - unfold tge. i.
-    exploit Genv_map_defs_def; et. i; des.
+  - unfold tge. i. exploit Genv_map_defs_def; et. i; des.
     uo. des_ifs. bsimpl.
     exploit SIMDEFINV; et. i; des. clarify. psimpl. clear_tac.
     exploit Genv.invert_find_symbol; et. intro SYMBTGT; des.
@@ -127,18 +116,13 @@ Proof.
       ii. des. align_bool; bsimpl. des_sumbool. ss. des; clarify.
       unfold defs in *. des_sumbool. ss.
     }
-    i; des.
-    clarify. clear_tac.
+    i; des. clarify. clear_tac.
 
     assert(blk_src = b).
     { eapply DISJ; et. }
     clarify.
 
-    unfold ge.
-    unfold SkEnv.revive.
-    erewrite Genv_map_defs_def_inv; et.
-    uo.
-    des_ifs_safe.
+    unfold ge. unfold SkEnv.revive. erewrite Genv_map_defs_def_inv; et. uo. des_ifs_safe.
 
     hexploit (match_prog_def _ _ _ TRANSL1 i); et. intro DEFMAP. des_ifs.
   - eauto.
@@ -148,10 +132,7 @@ Qed.
 Let SEGESRC: senv_genv_compat skenv_link_src ge. Proof. eapply SkEnv.senv_genv_compat; et. Qed.
 Let SEGETGT: senv_genv_compat skenv_link_tgt tge. Proof. eapply SkEnv.senv_genv_compat; et. Qed.
 
-Theorem sim_modsem
-  :
-    ModSemPair.sim msp
-.
+Theorem sim_modsem: ModSemPair.sim msp.
 Proof.
   (* rr in TRANSL. destruct TRANSL as [TRANSL0 TRANSL1]. *)
   destruct TRANSL as [used0 TRANSL0]. des.
@@ -164,24 +145,17 @@ Proof.
   - (* init bsim *)
     (* destruct sm_arg; ss. clarify. *)
     destruct args_src, args_tgt; ss.
-    inv SIMARGS; ss. clarify.
-    inv INITTGT. ss.
+    inv SIMARGS; ss. clarify. inv INITTGT. ss.
     assert(SIMGE: meminj_preserves_globals prog tprog (used_set tprog) ge tge (SimMemInj.inj sm_arg)).
     { eapply sim_skenv_meminj_preserves_globals; et. apply SIMSKENV. }
-    des.
-    eexists.
+    des. eexists.
     
     exploit SimMemInjC.inject_junk_blocks_tgt; et. intro P; des.
-    exists sm1.
-    esplits; eauto.
+    exists sm1. esplits; eauto.
     + econs; eauto; ss; cycle 1.
       { inv SAFESRC. ss. }
       { rewrite DEF. ss. }
-      * inv TYP.
-        inv SAFESRC. folder. ss.
-
-
-        inv TYP.
+      * inv TYP. inv SAFESRC. folder. ss. inv TYP.
         exploit find_funct_inject; et. i; des. clarify.
         rpapply match_states_call; ss; eauto.
         { econs; ss; et.
@@ -191,16 +165,13 @@ Proof.
         }
         { eapply inject_list_typify_list; eauto. }
         { eapply MWF0. }
-  - des. inv SAFESRC.
-    inv SIMARGS; ss.
+  - des. inv SAFESRC. inv SIMARGS; ss.
     assert(SIMGE: meminj_preserves_globals prog tprog (used_set tprog) ge tge (SimMemInj.inj sm_arg)).
     { eapply sim_skenv_meminj_preserves_globals; et. apply SIMSKENV. }
-    exploit find_funct_inject; et. i; des. clarify.
-    inv TYP.
+    exploit find_funct_inject; et. i; des. clarify. inv TYP.
     esplits; eauto. econs; eauto.
     + (* TODO: add lemma *)
-      econs; et.
-      etrans; try apply LEN; et. symmetry. eapply inject_list_length; et.
+      econs; et. etrans; try apply LEN; et. symmetry. eapply inject_list_length; et.
     + etrans; try apply LEN; et. symmetry. eapply inject_list_length; et.
   - (* call wf *)
     inv MATCH; ss. inv MATCHST; ss.
@@ -208,38 +179,30 @@ Proof.
     des. clear_tac.
     assert(SIMGE: meminj_preserves_globals prog tprog (used_set tprog) ge tge (SimMemInj.inj sm0)).
     { eapply sim_skenv_meminj_preserves_globals; et. apply SIMSKENV. }
-    inv MATCH; ss.
-    inv CALLSRC. inv MATCHST; ss. clarify.
-    folder.
-    inv MCOMPAT; ss. clear_tac.
-    inv FPTR; try (by des; ss).
-    ss. destruct (Ptrofs.eq_dec ofs1 Ptrofs.zero); clarify; try (by des; ss).
+    inv MATCH; ss. inv CALLSRC. inv MATCHST; ss. clarify.
+    folder. inv MCOMPAT; ss. clear_tac.
+    inv FPTR; try (by des; ss). ss. destruct (Ptrofs.eq_dec ofs1 Ptrofs.zero); clarify; try (by des; ss).
     esplits; try refl; eauto.
     + econs; eauto.
-      * folder.
-        ss. des_ifs_safe.
+      * folder. ss. des_ifs_safe.
         inv SIMGE. uge0. des_ifs_safe. exploit defs_rev_inject; eauto. i; des. clarify. des_ifs_safe. des_ifs.
       * clear EXTERNAL. des. ss. uge0. des_ifs_safe.
-        psimpl.
-        inv SIMSKENV. inv SIMSKELINK. ss.
+        psimpl. inv SIMSKENV. inv SIMSKELINK. ss.
         exploit SIMDEF; et. i; des. clarify. des_ifs. esplits; et.
     + econs; ss; et.
   - (* after fsim *)
     des. clear_tac.
     assert(SIMGE: meminj_preserves_globals prog tprog (used_set tprog) ge tge (SimMemInj.inj sm0)).
     { eapply sim_skenv_meminj_preserves_globals; et. apply SIMSKENV. }
-    inv AFTERSRC.
-    inv SIMRET. ss. exists (SimMemInj.unlift' sm_arg sm_ret).
+    inv AFTERSRC. inv SIMRET. ss. exists (SimMemInj.unlift' sm_arg sm_ret).
     inv MATCH; ss. inv MATCHST; ss.
     inv HISTORY. ss. clear_tac.
     esplits; try refl; eauto.
     + econs; eauto.
     + econs; ss; eauto. destruct retv_src, retv_tgt; ss. clarify.
-      inv MLE0; ss.
-      inv MCOMPAT. clear_tac.
+      inv MLE0; ss. inv MCOMPAT. clear_tac.
       rpapply match_states_return; ss; eauto; ss.
-      {
-        eapply match_stacks_bound; et; cycle 1.
+      { eapply match_stacks_bound; et; cycle 1.
         { eauto with mem. }
         { eauto with mem. }
         eapply match_stacks_incr; et.
@@ -249,8 +212,7 @@ Proof.
       { eapply MWFAFTR. }
 
   - (* final fsim *)
-    inv MATCH. inv FINALSRC; inv MATCHST; ss.
-    inv STACKS. inv MCOMPAT; ss.
+    inv MATCH. inv FINALSRC; inv MATCHST; ss. inv STACKS. inv MCOMPAT; ss.
     eexists sm0. esplits; ss; eauto. refl.
   - (* step *)
     left; i.
@@ -259,14 +221,11 @@ Proof.
 
     esplits; eauto.
     { apply modsem_receptive; et. }
-    inv MATCH.
-    ii. hexploit (@step_simulation prog tprog (used_set tprog) skenv_link_src skenv_link_tgt); eauto.
-    i; des.
+    inv MATCH. ii.
+    hexploit (@step_simulation prog tprog (used_set tprog) skenv_link_src skenv_link_tgt); eauto. i; des.
     esplits; eauto.
     + left. apply plus_one. econs; eauto. eapply modsem2_determinate; eauto.
-    + econs; ss.
-      * inv H0; ss; inv MCOMPAT; ss.
-      * inv H0; ss; inv MCOMPAT; ss.
+    + econs; ss; inv H0; ss; inv MCOMPAT; ss.
 Unshelve.
   all: ss; try (by econs).
 Qed.
@@ -281,13 +240,9 @@ Variable tprog: RTL.program.
 Hypothesis TRANSL: match_prog prog tprog.
 
 Definition mp: ModPair.t :=
-  ModPair.mk (RTLC.module prog) (RTLC.module2 tprog) ((prog.(defs) -1 tprog.(defs) -1 (Pos.eq_dec tprog.(prog_main))): ident -> Prop)
-.
+  ModPair.mk (RTLC.module prog) (RTLC.module2 tprog) ((prog.(defs) -1 tprog.(defs) -1 (Pos.eq_dec tprog.(prog_main))): ident -> Prop).
 
-Theorem sim_mod
-  :
-    ModPair.sim mp
-.
+Theorem sim_mod: ModPair.sim mp.
 Proof.
   econs; ss.
   - destruct TRANSL as [used0 TRANSL0]. desH TRANSL0. clarify.
@@ -298,8 +253,7 @@ Proof.
       generalize (Sk.of_program_prog_defmap tprog fn_sig id). intro REL1.
 
       destruct (classic (defs prog id)); cycle 1.
-      {
-        rewrite <- (Sk.of_program_defs fn_sig) in H.
+      { rewrite <- (Sk.of_program_defs fn_sig) in H.
         inv REL0; align_opt; cycle 1.
         { exploit prog_defmap_image; et. i; des. unfold defs in *. align_bool; bsimpl. align_bool. des_sumbool. ss. }
         unfold fundef in *.
@@ -318,8 +272,7 @@ Proof.
         - des_sumbool. clarify. tauto.
       }
 
-      des_ifs.
-      unfold fundef in *. rewrite match_prog_def in *.
+      des_ifs. unfold fundef in *. rewrite match_prog_def in *.
       erewrite (Sk.of_program_prog_defmap_eq fn_sig prog tprog) in *; ss.
 
     + i. ss. inv TRANSL1.
@@ -334,8 +287,7 @@ Proof.
 
     + ii. unfold privs. bsimpl. des. bsimpl. des_sumbool.
       rewrite (Sk.of_program_defs fn_sig). split; ss.
-      unfold NW. align_bool; bsimpl. des_sumbool.
-      ii.
+      unfold NW. align_bool; bsimpl. des_sumbool. ii.
 
       exploit used_public; et. intro IN. unfold used_set in IN. des_sumbool. ss. des; clarify; ss.
       unfold defs in *. des_sumbool. ss.
@@ -343,18 +295,15 @@ Proof.
     + inv TRANSL1; ss.
 
     + inv TRANSL1; ss.
-    + ii. des.
-      inv TRANSL0.
+    + ii. des. inv TRANSL0.
       assert(PROG0: (prog_defmap tprog) ! id = Some (Gvar gv)).
-      {
-        (* TODO: make lemma!!!!!!!!!!!!!!!!!!! *)
+      { (* TODO: make lemma!!!!!!!!!!!!!!!!!!! *)
         generalize (Sk.of_program_prog_defmap tprog fn_sig id). intro REL.
         inv REL; try congruence.
         rewrite PROG in *. clarify.
         inv H2. inv H4. ss. destruct i1, i2; ss.
       }
-      inv TRANSL1.
-      rewrite match_prog_def in *. des_ifs.
+      inv TRANSL1. rewrite match_prog_def in *. des_ifs.
       exploit (used_closed id); et. ii.
       exploit used_defined; et. i; des.
       { exploit prog_defmap_dom; et. i; des. specialize (match_prog_def id_drop). des_ifs. rewrite H2 in *.
