cfrontend/CshmgenproofC.v
@@ -50,18 +50,14 @@ Inductive match_states
 | match_states_intro
     (MATCHST: Cshmgenproof.match_states prog ge st_src0 st_tgt0)
     (MCOMPATSRC: st_src0.(ClightC.get_mem) = sm0.(SimMem.src))
-    (MCOMPATTGT: st_tgt0.(CsharpminorC.get_mem) = sm0.(SimMem.tgt))
-.
+    (MCOMPATTGT: st_tgt0.(CsharpminorC.get_mem) = sm0.(SimMem.tgt)).
 
 Theorem make_match_genvs :
   SimSymbId.sim_skenv (SkEnv.project skenv_link md_src.(Mod.sk)) (SkEnv.project skenv_link md_tgt.(Mod.sk)) ->
   Genv.match_genvs (match_globdef match_fundef match_varinfo prog) ge tge.
 Proof. subst_locals. ss. eapply SimSymbId.sim_skenv_revive; eauto. Qed.
 
-Theorem sim_modsem
-  :
-    ModSemPair.sim msp
-.
+Theorem sim_modsem: ModSemPair.sim msp.
 Proof.
   eapply match_states_sim with (match_states := match_states) (match_states_at := top4)
                                (sound_state := SoundTop.sound_state);
@@ -70,31 +66,24 @@ Proof.
   - eapply SoundTop.sound_state_local_preservation.
   - (* init bsim *)
     destruct sm_arg; ss. clarify.
-    inv SIMARGS; ss. clarify.
-    inv INITTGT.
+    inv SIMARGS; ss. clarify. inv INITTGT.
     exploit make_match_genvs; eauto. { apply SIMSKENV. } intro SIMGE. des.
-    eexists. eexists (SimMemId.mk _ _).
-    esplits; eauto.
+    eexists. eexists (SimMemId.mk _ _). esplits; eauto.
     + econs; eauto; ss.
-      * inv TYP.
-        inv SAFESRC. folder.
+      * inv TYP. inv SAFESRC. folder.
         rpapply match_callstate; eauto.
         { econs; eauto. }
         { ss. }
         inv TYP.
         exploit (Genv.find_funct_match_genv SIMGE); eauto. intro FINDFSRC; des.
         rewrite <- FPTR in *. clarify.
-        inv FINDFSRC0.
-        monadInv H1; ss.
-        f_equal; try congruence.
+        inv FINDFSRC0. monadInv H1; ss. f_equal; try congruence.
         { exploit (function_type_implies_sig fd0); et. unfold type_of_function. ss. }
   - (* init progress *)
-    des. inv SAFESRC.
-    inv SIMARGS; ss.
+    des. inv SAFESRC. inv SIMARGS; ss.
     exploit make_match_genvs; eauto. { apply SIMSKENV. } intro SIMGE.
     exploit (Genv.find_funct_match_genv SIMGE); eauto. i; des. ss. clarify. folder.
-    inv TYP.
-    inv H0. ss.
+    inv TYP. inv H0. ss.
     assert(TYEQ: (ClightC.signature_of_function fd) = fn_sig tf0).
     { monadInv H3. ss. }
     esplits; eauto. econs; eauto.
@@ -102,45 +91,34 @@ Proof.
     + rewrite <- VALS. econs; eauto with congruence. rewrite <- TYEQ. ss.
     + rewrite <- VALS. rewrite <- TYEQ. ss.
   - (* call wf *)
-    inv MATCH; ss. destruct sm0; ss. clarify.
-    inv CALLSRC. inv MATCHST; ss.
+    inv MATCH; ss. destruct sm0; ss. clarify. inv CALLSRC. inv MATCHST; ss.
   - (* call fsim *)
-    inv MATCH; ss. destruct sm0; ss. clarify.
-    inv CALLSRC. inv MATCHST; ss.
-    folder.
-    esplits; eauto.
+    inv MATCH; ss. destruct sm0; ss. clarify. inv CALLSRC. inv MATCHST; ss.
+    folder. esplits; eauto.
     + econs; eauto.
-      * folder. des.
-        r in TRANSL.
+      * folder. des. r in TRANSL.
         exploit (SimSymbId.sim_skenv_revive TRANSL); eauto.
         { apply SIMSKENV. }
-        intro GE.
-        apply (fsim_external_funct_id GE); ss.
+        intro GE. apply (fsim_external_funct_id GE); ss.
       * des. clarify. esplits; eauto.
     + econs; ss; eauto.
       * instantiate (1:= SimMemId.mk _ _). ss.
       * ss.
     + ss.
   - (* after fsim *)
-    inv AFTERSRC.
-    inv SIMRET. ss. exists sm_ret. destruct sm_ret; ss. clarify.
-    inv MATCH; ss. inv MATCHST; ss.
-    esplits; eauto.
+    inv AFTERSRC. inv SIMRET. ss. exists sm_ret. destruct sm_ret; ss. clarify.
+    inv MATCH; ss. inv MATCHST; ss. esplits; eauto.
     + econs; eauto.
     + econs; ss; eauto. destruct retv_src, retv_tgt; ss. clarify.
       rpapply match_returnstate; eauto. repeat f_equal. rewrite proj_sig_res_type. ss.
   - (* final fsim *)
-    inv MATCH. inv FINALSRC; inv MATCHST; ss.
-    inv MK; ss. destruct sm0; ss. clarify.
+    inv MATCH. inv FINALSRC; inv MATCHST; ss. inv MK; ss. destruct sm0; ss. clarify.
     eexists (SimMemId.mk _ _). esplits; ss; eauto.
-  - left; i.
-    esplits; eauto.
+  - left; i. esplits; eauto.
     { apply modsem2_receptive. }
-    inv MATCH.
-    ii. hexploit (@transl_step prog skenv_link skenv_link); eauto; ss.
+    inv MATCH. ii. hexploit (@transl_step prog skenv_link skenv_link); eauto; ss.
     { apply make_match_genvs; eauto. apply SIMSKENV. }
-    i; des.
-    esplits; eauto.
+    i; des. esplits; eauto.
     + left. eapply spread_dplus; eauto. eapply modsem_determinate; eauto.
     + instantiate (1:= SimMemId.mk _ _). econs; ss.
 Unshelve.
@@ -157,10 +135,7 @@ Variable tprog: Csharpminor.program.
 Hypothesis TRANSL: match_prog prog tprog.
 Definition mp: ModPair.t := ModPair.mk (ClightC.module2 prog) (CsharpminorC.module tprog) tt.
 
-Theorem sim_mod
-  :
-    ModPair.sim mp
-.
+Theorem sim_mod: ModPair.sim mp.
 Proof.
   econs; ss.
   - r. inv TRANSL. des. unfold CSk.of_program, Sk.of_program. f_equal; ss.
@@ -168,12 +143,9 @@ Proof.
     destruct prog, tprog; ss. clear - H.
     ginduction prog_defs; ii; ss; inv H; ss.
     erewrite IHprog_defs; et. f_equal; ss.
-    inv H2. destruct a, b1; ss. clarify.
-    inv H0; ss.
-    + unfold update_snd. ss. f_equal.
-      destruct f1.
-      * inv H1. unfold transl_function in H2. unfold bind in *. ss. des_ifs.
-      * inv H1. ss.
+    inv H2. destruct a, b1; ss. clarify. inv H0; ss.
+    + unfold update_snd. ss. f_equal. destruct f1; inv H1; ss.
+      unfold transl_function in H2. unfold bind in *. ss. des_ifs.
     + inv H. ss.
   - ii. inv SIMSKENVLINK. eapply sim_modsem; eauto.
 Qed.
