cfrontend/CtypesC.v
@@ -17,8 +17,7 @@ Definition fundef_of_fundef F (f: Ctypes.fundef F): AST.fundef F :=
   match f with
   | Internal f => AST.Internal f
   | External ef _ _ _ => AST.External ef
-  end
-.
+  end.
 
 Coercion fundef_of_fundef: Ctypes.fundef >-> AST.fundef.
 
@@ -35,16 +34,11 @@ Global Instance fundef_HasExternal {F}: HasExternal (Ctypes.fundef F) :=
 Module CSk.
 
   Definition of_program {F} (get_sg: F -> signature) (prog: Ctypes.program F): Sk.t :=
-    mkprogram (skdefs_of_gdefs get_sg (map (update_snd (@globdef_of_globdef F type)) prog.(prog_defs))) prog.(prog_public) prog.(prog_main)
-  .
+    mkprogram (skdefs_of_gdefs get_sg (map (update_snd (@globdef_of_globdef F type)) prog.(prog_defs))) prog.(prog_public) prog.(prog_main).
 
   Lemma of_program_defs
-        F
-        get_sg
-        (p: Ctypes.program F)
-    :
-      (of_program get_sg p).(defs) = p.(defs)
-  .
+        F get_sg (p: Ctypes.program F):
+      (of_program get_sg p).(defs) = p.(defs).
   Proof.
     destruct p; ss.
     Local Opaque in_dec.
@@ -61,71 +55,51 @@ Module CSk.
       | Internal func0, AST.Internal func1 => get_sig func0 = func1
       | External ef0 _ _ _, AST.External ef1 => external_function_eq ef0 ef1
       | _, _ => false
-      end
-  .
+      end.
 
   (* copied from Skeleton *)
   Definition wf_match_fundef CTX F1 F2 (match_fundef: CTX -> Ctypes.fundef F1 -> Ctypes.fundef F2 -> Prop)
              (fn_sig1: F1 -> signature) (fn_sig2: F2 -> signature): Prop := forall
       ctx f1 f2
-      (MATCH: match_fundef ctx f1 f2)
-    ,
+      (MATCH: match_fundef ctx f1 f2),
       (<<EXT: exists ef targs tres cc, f1 = External ef targs tres cc /\ f2 = External ef targs tres cc>>)
-      \/ (<<INT: exists fd1 fd2, f1 = Internal fd1 /\ f2 = Internal fd2 /\ <<SIG: fn_sig1 fd1 = fn_sig2 fd2>> >>)
-  .
+      \/ (<<INT: exists fd1 fd2, f1 = Internal fd1 /\ f2 = Internal fd2 /\ <<SIG: fn_sig1 fd1 = fn_sig2 fd2>> >>).
 
   Lemma match_program_eq
-        F1 F2
+        F1 F2 match_fundef match_varinfo fn_sig1 fn_sig2
         `{Linker (Ctypes.fundef F1)}
-        match_fundef match_varinfo
         (p1: Ctypes.program F1)
         (p2: Ctypes.program F2)
         (MATCH: match_program match_fundef match_varinfo p1 p2)
-        fn_sig1 fn_sig2
-        (WF: wf_match_fundef match_fundef fn_sig1 fn_sig2)
-    :
-      <<EQ: CSk.of_program fn_sig1 p1 = CSk.of_program fn_sig2 p2>>
-  .
+        (WF: wf_match_fundef match_fundef fn_sig1 fn_sig2):
+      <<EQ: CSk.of_program fn_sig1 p1 = CSk.of_program fn_sig2 p2>>.
   Proof.
     rr in MATCH. des.
     unfold of_program. r. f_equal; ss.
     revert MATCH. generalize p1 at 1 as CTX. i.
-    destruct p1, p2; ss.
-    clear - MATCH WF.
+    destruct p1, p2; ss. clear - MATCH WF.
     ginduction prog_defs; ii; ss; inv MATCH; ss.
     erewrite IHprog_defs; eauto. f_equal; eauto.
-    inv H2. destruct a, b1; ss. clarify.
-    inv H1; ss.
+    inv H2. destruct a, b1; ss. clarify. inv H1; ss.
     - unfold update_snd. exploit WF; eauto. i; des; clarify; ss.
       + repeat f_equal. exploit WF; et.
     - inv H0. ss.
   Qed.
 
-  Lemma of_program_prog_defmap
-        F
-        (p: Ctypes.program F)
-        (get_sg: F -> signature)
-    :
+  Lemma of_program_prog_defmap: forall F (p: Ctypes.program F) (get_sg: F -> signature),
       <<SIM: forall id, option_rel (@Linking.match_globdef unit _ _ _ _ _
                                                            (@match_fundef _ _ get_sg)
                                                            top2
                                                            tt)
-                                   (p.(prog_defmap) ! id) ((of_program get_sg p).(prog_defmap) ! id)>>
-  .
+                                   (p.(prog_defmap) ! id) ((of_program get_sg p).(prog_defmap) ! id)>>.
   Proof.
-    ii.
-    unfold prog_defmap, of_program, skdefs_of_gdefs. ss.
-    rewrite prog_defmap_update_snd.
-    rewrite prog_defmap_update_snd.
+    ii. unfold prog_defmap, of_program, skdefs_of_gdefs. ss.
+    rewrite prog_defmap_update_snd. rewrite prog_defmap_update_snd.
     destruct ((PTree_Properties.of_list (prog_defs p)) ! id) eqn:T; ss.
     - econs; et. unfold skdef_of_gdef.
       destruct g; ss; clarify; unfold fundef_of_fundef in *; des_ifs.
-      + econs; et.
-        { refl. }
-        econs; et.
-      + econs; et.
-        { refl. }
-        r. des_sumbool. refl.
+      + econs; et; ss.
+      + econs; et; ss. r. des_sumbool. refl.
       + econs; et. destruct v; ss.
     - econs; et.
   Unshelve.
@@ -133,22 +107,14 @@ Module CSk.
   Qed.
   Local Opaque prog_defmap.
 
-  Lemma of_program_internals
-        F
-        get_sg
-        (p: Ctypes.program F)
-    :
-      (of_program get_sg p).(internals) = p.(internals)
-  .
+  Lemma of_program_internals: forall F get_sg (p: Ctypes.program F),
+      (of_program get_sg p).(internals) = p.(internals).
   Proof.
-    unfold internals.
-    destruct p; ss.
-    apply Axioms.functional_extensionality. intro id; ss.
-    u.
+    unfold internals. destruct p; ss.
+    apply Axioms.functional_extensionality. intro id; ss. u.
     exploit (of_program_prog_defmap). i. inv H.
     - rewrite <- H2. rewrite <- H1. ss.
-    - des_ifs_safe. inv H2; ss. unfold match_fundef in *. des_ifs. des_sumbool. clarify.
-      ss. clarify.
+    - des_ifs_safe. inv H2; ss. unfold match_fundef in *. des_ifs. des_sumbool. clarify. ss. clarify.
   Qed.
   Local Transparent prog_defmap.
 
@@ -160,29 +126,20 @@ Module CSkEnv.
   Local Opaque prog_defs_names.
   Local Opaque prog_defmap.
   Lemma project_revive_precise
-        F
-        skenv (prog: Ctypes.program F)
+        F skenv (prog: Ctypes.program F) skenv_link get_sg
         (* (DEFS0: forall id, In id prog.(prog_defs_names) -> is_some (skenv.(Genv.find_symbol) id)) *)
         (* (WF: wf skenv) *)
-        skenv_link
         (* (PROJ: skenv = SkEnv.project skenv_link prog) *)
-        get_sg
         (PROJ: SkEnv.project_spec skenv_link prog.(CSk.of_program get_sg) skenv)
         (* (WF: SkEnv.wf skenv_link) *)
-        (INCL: SkEnv.includes skenv_link prog.(CSk.of_program get_sg))
-    (* (PRECISE: SkEnv.genv_precise (SkEnv.revive skenv prog) prog *)
-    :
-      <<PRECISE: SkEnv.genv_precise (SkEnv.revive skenv prog) prog>>
-  .
+        (* (PRECISE: SkEnv.genv_precise (SkEnv.revive skenv prog) prog *)
+        (INCL: SkEnv.includes skenv_link prog.(CSk.of_program get_sg)):
+      <<PRECISE: SkEnv.genv_precise (SkEnv.revive skenv prog) prog>>.
   Proof.
     assert(H: DUMMY_PROP) by ss.
     assert(DEFS: prog.(defs) <1= fun id => is_some (skenv.(Genv.find_symbol) id)).
     { ii; ss. u. des_ifs. exfalso.
-      bar.
-      inv PROJ.
-      bar.
-      inv INCL.
-      bar.
+      bar. inv PROJ. bar. inv INCL. bar.
       exploit SYMBKEEP; et.
       { rewrite CSk.of_program_defs. eauto. }
       intro EQ. des. rewrite Heq in *. symmetry in EQ.
@@ -191,39 +148,25 @@ Module CSkEnv.
       exploit DEFS; et. i; des. clarify.
     }
     econs; eauto; i; ss; cycle 1.
-    - des.
-      unfold SkEnv.revive in *.
+    - des. unfold SkEnv.revive in *.
       apply_all_once Genv_map_defs_def. des; ss.
       uo. des_ifs. esplits; et.
       + rewrite Genv_map_defs_symb. eapply Genv.invert_find_symbol; et.
-      + inv PROJ.
-        rewrite CSk.of_program_defs in *. rewrite CSk.of_program_internals in *.
+      + inv PROJ. rewrite CSk.of_program_defs in *. rewrite CSk.of_program_internals in *.
         assert(DEF: defs prog i).
         { u. des_sumbool. eapply prog_defmap_spec; et. }
         exploit DEFKEPT; et.
-        { eapply Genv.find_invert_symbol; et.
-          rewrite <- SYMBKEEP; et.
-          eapply Genv.invert_find_symbol; et.
-        }
-        intro T; des.
-        ss. rename g into gg. rename gd1 into gg1. bsimpl.
+        { eapply Genv.find_invert_symbol; et. rewrite <- SYMBKEEP; et. eapply Genv.invert_find_symbol; et. }
+        intro T; des. ss. rename g into gg. rename gd1 into gg1. bsimpl.
         unfold ASTC.internals in T. des_ifs. ss. unfold NW in *. bsimpl. congruence.
-    -
-      dup H. u in DEFS. unfold ident in *. spc DEFS.
+    - dup H. u in DEFS. unfold ident in *. spc DEFS.
       exploit DEFS; clear DEFS.
       { unfold proj_sumbool. des_ifs; ss. exfalso. apply n. eapply prog_defmap_spec; eauto. }
-      i; des.
-      des_ifs_safe.
-      esplits; eauto.
-      unfold SkEnv.revive. u.
-      unfold Genv.find_def, Genv_map_defs. cbn. rewrite PTree_filter_map_spec.
-      clear_tac.
-      rewrite o_bind_ignore.
+      i; des. des_ifs_safe. esplits; eauto.
+      unfold SkEnv.revive. u. unfold Genv.find_def, Genv_map_defs. cbn. rewrite PTree_filter_map_spec.
+      clear_tac. rewrite o_bind_ignore.
       exploit Genv.find_invert_symbol; et. intro INV.
-      bar.
-      inv PROJ.
-      inv INCL.
-      bar.
+      bar. inv PROJ. inv INCL. bar.
       assert(defs (CSk.of_program get_sg prog) id).
       { apply NNPP. ii. exploit SYMBDROP; et. i; des. clarify. }
       exploit SYMBKEEP; et. intro SYMBLINK; des. rewrite Heq in *. symmetry in SYMBLINK.
@@ -232,18 +175,13 @@ Module CSkEnv.
       rewrite PROG in *. inv REL.
       rename H2 into MATCHGD. rename H1 into DEFMAP1.
       exploit DEFS; et. i; des. clarify.
-      des_ifs_safe.
-      inv MATCHGD; cycle 1.
-      {
-        des_ifs_safe.
-        inv MATCH.
+      des_ifs_safe. inv MATCHGD; cycle 1.
+      { des_ifs_safe. inv MATCH.
         exploit DEFKEEP; et.
         { rewrite CSk.of_program_internals. u. des_ifs. }
         i; des. uge. clarify.
       }
-      {
-        inv MATCH.
-        destruct (is_external_fd f1) eqn:T.
+      { inv MATCH. destruct (is_external_fd f1) eqn:T.
         - etrans; cycle 1.
           { instantiate (1:= None). des_ifs. ss. des_ifs. }
           assert(is_external f2).
@@ -252,8 +190,7 @@ Module CSkEnv.
           rename f2 into fd_small. rename f1 into fd_small2.
           (* if (Genv.genv_defs skenv) is some, then it should be fd_big *)
           (* fd_big *)
-          bar.
-          des_ifs. uge.
+          bar. des_ifs. uge.
           exploit DEFKEPT; et. i; des. clarify.
           rewrite CSk.of_program_internals in *.
           u in H4. des_ifs. bsimpl. ss. clarify.
@@ -268,42 +205,34 @@ Module CSkEnv.
   Qed.
 
   Lemma project_revive_no_external
-        F (prog: Ctypes.program F)
-        skenv_link get_sg blk gd
+        F (prog: Ctypes.program F) skenv_link get_sg blk gd
         (DEF: Genv.find_def (SkEnv.revive (SkEnv.project skenv_link (CSk.of_program get_sg prog)) prog) blk = Some gd)
         (EXTERNAL: is_external gd)
         (INCL: SkEnv.includes skenv_link (CSk.of_program get_sg prog))
-        (WF: SkEnv.wf skenv_link)
-    :
-      False
-  .
+        (WF: SkEnv.wf skenv_link):
+      False.
   Proof.
     assert(H: DUMMY_PROP) by ss.
     hexploit (@SkEnv.project_impl_spec skenv_link (CSk.of_program get_sg prog)); et. intro PROJ. des.
     exploit project_revive_precise; et. intro GEP; des.
     exploit SkEnv.project_spec_preserves_wf; et. intro WF0; des.
-    inv WF0.
-    dup DEF.
+    inv WF0. dup DEF.
     unfold SkEnv.revive in DEF. apply Genv_map_defs_def in DEF. des.
     exploit DEFSYMB; et. i; des.
     inv GEP.
     exploit GE2P.
     { esplits; et. }
-    i; des.
-    uo. des_ifs.
+    i; des. uo. des_ifs.
   Qed.
 
   Lemma senv_genv_compat
         F (skenv_link: SkEnv.t) fn_sig (prog: Ctypes.program F)
-        (INCL: SkEnv.includes skenv_link (CSk.of_program fn_sig prog))
-    :
-      senv_genv_compat skenv_link (SkEnv.revive (SkEnv.project skenv_link (CSk.of_program fn_sig prog)) prog)
-  .
+        (INCL: SkEnv.includes skenv_link (CSk.of_program fn_sig prog)):
+      senv_genv_compat skenv_link (SkEnv.revive (SkEnv.project skenv_link (CSk.of_program fn_sig prog)) prog).
   Proof.
     exploit CSkEnv.project_revive_precise; eauto.
     { eapply SkEnv.project_impl_spec; eauto. }
-    intro PREC.
-    econs; eauto. i. ss.
+    intro PREC. econs; eauto. i. ss.
     (* inv INCL. inv PREC. *)
     ss. uge. unfold SkEnv.revive in *. ss. rewrite MapsC.PTree_filter_key_spec in *. des_ifs.
   Qed.
