backend/LineartypingC.v
@@ -30,19 +30,14 @@ Lemma ls_init_has_type
       (LOCSET: typify_list vs sg = map (fun p => Locmap.getpair p ls_init) (loc_arguments_64 sg ir fr ofs))
       sl pos ty
       (IN: In (S sl pos ty) (regs_of_rpairs (loc_arguments_64 sg ir fr ofs)))
-      (ONES: forall lp, In lp (loc_arguments_64 sg ir fr ofs) -> is_one lp)
-  :
-    <<TY: Val.has_type (ls_init (S sl pos ty)) ty>>
-.
+      (ONES: forall lp, In lp (loc_arguments_64 sg ir fr ofs) -> is_one lp):
+    <<TY: Val.has_type (ls_init (S sl pos ty)) ty>>.
 Proof.
   remember (loc_arguments_64 sg ir fr ofs) as locs in *.
   Local Opaque Z.add Z.mul Z.sub Z.div.
   Local Opaque loc_arguments_64.
-  ginduction locs; ii; ss. destruct vs; ss. destruct sg; ss. clarify.
-  unfold typify_list in *.
-  exploit ONES; eauto. i. destruct a; ss.
-  clarify.
-  des; cycle 1.
+  ginduction locs; ii; ss. destruct vs; ss. destruct sg; ss. clarify. unfold typify_list in *.
+  exploit ONES; eauto. i. destruct a; ss. clarify. des; cycle 1.
   - Local Transparent loc_arguments_64.
     ss. des_ifs; eapply IHlocs; eauto.
   - clarify. rewrite <- H3.
@@ -58,32 +53,16 @@ Section SOUNDNESS.
   Variable prog: program.
 
   Hypothesis wt_prog:
-    forall i fd, In (i, Gfun fd) prog.(prog_defs) -> wt_fundef fd
-  .
+    forall i fd, In (i, Gfun fd) prog.(prog_defs) -> wt_fundef fd.
 
-  Lemma mreg_type_any
-        mr
-    :
-      <<ANY: mreg_type mr = Tany64>>
-  .
-  Proof.
-    unfold mreg_type. des_ifs.
-  Qed.
+  Lemma mreg_type_any: forall mr, <<ANY: mreg_type mr = Tany64>>.
+  Proof. i. rr. unfold mreg_type. des_ifs. Qed.
 
-  Lemma has_type_any
-        v
-    :
-      <<ANY: Val.has_type v Tany64>>
-  .
-  Proof.
-    destruct v; ss.
-  Qed.
+  Lemma has_type_any: forall v, <<ANY: Val.has_type v Tany64>>.
+  Proof. i. rr. destruct v; ss. Qed.
 
-  Theorem wt_state_local_preservation
-          skenv_link
-    :
-      local_preservation (modsem skenv_link prog) (fun _ _ st => wt_state st)
-  .
+  Theorem wt_state_local_preservation: forall skenv_link,
+      local_preservation (modsem skenv_link prog) (fun _ _ st => wt_state st).
   Proof.
     econs; ii; ss; eauto.
     - (* init *)
@@ -93,44 +72,34 @@ Section SOUNDNESS.
         destruct l; ss.
         { rewrite mreg_type_any. apply has_type_any. }
         destruct (classic (In (S sl pos ty) (regs_of_rpairs (loc_arguments (fn_sig fd))))).
-        - clear - TYP H.
-          inv TYP.
-          abstr (fn_sig fd) sg.
-          abstr (Args.vs args) vs. clear_tac.
+        - clear - TYP H. inv TYP.
+          abstr (fn_sig fd) sg. abstr (Args.vs args) vs. clear_tac.
           generalize (loc_arguments_one sg). intro ONES.
           destruct sg; ss. unfold loc_arguments in *. ss. des_ifs. clear_tac.
           eapply ls_init_has_type; eauto.
         - erewrite SLOT; eauto.
       }
-      econs; ss; eauto.
-      econs; eauto.
-      econs; eauto.
-    - inv STEP.
-      eapply step_type_preservation; eauto.
+      econs; ss; eauto. econs; eauto. econs; eauto.
+    - inv STEP. eapply step_type_preservation; eauto.
       ii. unfold Genv.find_funct, Genv.find_funct_ptr in *. des_ifs.
       unfold Skeleton.SkEnv.revive in *.
       eapply Genv_map_defs_def in Heq. des. u in MAP. des_ifs_safe. bsimpl.
       esplits. eapply in_prog_defmap; eauto.
     - esplits; eauto.
       { rr. esplits; ss; eauto. rr. rewrite Forall_forall. ii; ss. }
-      ii.
-      inv AFTER.
-      inv SUST.
+      ii. inv AFTER. inv SUST.
 
       hexploit (loc_result_caller_save sg_arg); eauto. intro RES.
       hexploit (loc_result_one sg_arg); eauto. intro ONE.
 
       econs; eauto.
-      + destruct stack; ss.
-        des_ifs. inv WTSTK.
-        econs; eauto.
-        unfold undef_outgoing_slots. ii. des_ifs.
+      + destruct stack; ss. des_ifs. inv WTSTK.
+        econs; eauto. unfold undef_outgoing_slots. ii. des_ifs.
       + ii. unfold Locmap.setpair. des_ifs. ss.
         apply wt_setreg; ss; cycle 1.
         { apply wt_undef_caller_save_regs; ss. }
         rewrite mreg_type_any. apply has_type_any.
-      + ii.
-        destruct l; ss.
+      + ii. destruct l; ss.
         { rewrite locmap_get_set_loc_result; ss. des_ifs. rewrite AGCS; ss.
           hexploit (parent_locset_after_external stack); et. i; des; clarify. rewrite AFTER.
           (* TODO: we can remove spurious case by strengthening wt_callstack -> *)
@@ -139,9 +108,7 @@ Section SOUNDNESS.
         }
         { rewrite locmap_get_set_loc_result; ss. rewrite AGCS; ss.
           hexploit (parent_locset_after_external stack); et. i.
-          des_ifs; des; clarify.
-          - rewrite AFTER; ss.
-          - rewrite AFTER; ss.
+          des_ifs; des; clarify; rewrite AFTER; ss.
         }
       + ii. rewrite locmap_get_set_loc_result; ss.
     - esplits; eauto. ss.
